certicoq/theories/L4_deBruijn/expression.v
@@ -1,0 +1,1262 @@
+Require Import Arith BinNat String List Omega Program Psatz.
+Open Scope N_scope.
+Opaque N.add.
+Opaque N.sub.
+
+(** A tactic for simplifying numeric tests. *)
+Ltac if_split := 
+  match goal with
+    | [ |- context[if ?e then _ else _] ] => 
+      destruct e; simpl; try lia; auto; try subst
+  end.
+
+Class Eq (A:Type) :=
+  {
+    eq_dec: forall (x y:A), {x = y} + {x<>y}
+  }.
+
+(** using [N] instead of [nat] **)
+Instance NEq: Eq N := { eq_dec := N.eq_dec }.
+Instance NatEq: Eq nat := { eq_dec := eq_nat_dec }.
+
+Definition lt_dec (x y:N): {x < y} + { x >= y}.
+  refine (match x <? y as z return (x <? y) = z -> {x < y} + {x >= y} with
+            | true => fun H => left _ (proj1 (N.ltb_lt x y) H)
+            | false => fun H => right _
+          end eq_refl).
+  intro. unfold N.ltb in *. rewrite H0 in H. discriminate.
+Defined.
+
+Lemma Nlt_or_ge: forall n m:N, n < m \/ m <= n.
+Proof. 
+  intros n m. lia.
+Qed.
+
+Lemma Nmax_plusr: forall x y, exists j, Nmax x y = j + y.
+Proof.
+  intros x y. destruct (N.max_spec x y) as [[h j]|[h j]].  
+  - exists 0. lia. 
+  - exists (x - y). replace (x - y + y) with x. assumption. lia.
+Qed.
+Lemma Nmax_plusl: forall x y, exists j, Nmax x y = j + x.
+Proof.
+  intros x y. replace (N.max x y) with (N.max y x); try lia.
+  apply Nmax_plusr.
+Qed.
+
+(**************************)
+(** * Source Expressions. *)
+(**************************)
+
+(* data constructors *)
+Definition dcon := N.
+Definition dcon0 := N0.
+
+(** Source expressions, represented using deBruijn notation *)
+Inductive exp: Type :=
+| Var_e: N -> exp
+| Lam_e: exp -> exp
+| App_e: exp -> exp -> exp
+| Con_e: dcon -> exps -> exp
+| Match_e: exp -> branches_e -> exp
+| Let_e: exp -> exp -> exp
+| Fix_e: efnlst -> exp  (* implicitly lambdas *)
+| Proj_e: exp -> N -> exp
+with exps: Type :=
+| enil: exps
+| econs: exp -> exps -> exps
+with efnlst: Type :=
+| eflnil: efnlst
+| eflcons: exp -> efnlst -> efnlst
+with branches_e: Type :=
+| brnil_e: branches_e
+| brcons_e: dcon -> N -> exp -> branches_e -> branches_e.
+Notation "[| e |]" := (econs e enil).
+Notation "[! f !]" := (eflcons f eflnil).
+Hint Constructors exp exps branches_e.
+Scheme exp_ind' := Induction for exp Sort Prop
+with exps_ind'  := Induction for exps Sort Prop
+with efnlst_ind'  := Induction for efnlst Sort Prop
+with branches_e_ind' := Induction for branches_e Sort Prop.
+Combined Scheme my_exp_ind from
+         exp_ind', exps_ind', efnlst_ind', branches_e_ind'.
+(* Notes on source expressions:  
+
+   [Let_e e1 e2] corresponds to (let x0 := e1 in e2)
+
+   [Fix_e [e1;e2;...;en]] produces an n-tuple of functions.  Each expression
+   is treated as binding (a) the n-tuple, and then (b) a function argument.
+   (Thus going under Fix_e increases index by 2).
+
+   So this is similar to saying something like:
+
+    let rec f1 = \x1.e1
+        and f2 = \x2.e2
+        ...
+        and fn = \xn.en
+    in
+      (f1,f2,...,fn)
+
+   When [e] evaluates to [Fix_e [e1;e2;...;en]], then [Proj_e e i] evaluates
+   to [ei{0 := Fix_e[e1;e2;...;en]}].  That is, we unwind the recursion when
+   you project something out of the tuple.
+
+   For [Match_e] each [branch], (d, n, e), binds [n] variables,
+   corresponding to the arguments to the data constructor d.  
+*)
+
+Fixpoint exps_length (es:exps) : N :=
+  match es with
+    | enil => N0
+    | econs _ es => 1 + (exps_length es)
+  end.
+
+(** Find the nth component in exps **)
+Fixpoint enthopt (n:nat) (xs:efnlst): option exp :=
+  match n, xs with 
+    | 0%nat, eflcons h _ => Some h
+    | S n, eflcons _ t => enthopt n t
+    | _, _ => None
+  end.
+
+(** [exp_wf i e] ensures there is no free variable above [i]. *)
+Inductive exp_wf: N -> exp -> Prop :=
+| var_e_wf: forall i j, j < i -> exp_wf i (Var_e j)
+| lam_e_wf: forall i e, exp_wf (1 + i) e -> exp_wf i (Lam_e e)
+| app_e_wf: forall i e1 e2, exp_wf i e1 -> exp_wf i e2 ->
+                             exp_wf i (App_e e1 e2)
+| con_e_wf: forall i d es, exps_wf i es -> exp_wf i (Con_e d es)
+| match_e_wf: forall i e bs, exp_wf i e -> branches_wf i bs ->
+                              exp_wf i (Match_e e bs)
+| let_e_wf: forall i e1 e2, exp_wf i e1 -> exp_wf (1 + i) e2 ->
+                             exp_wf i (Let_e e1 e2)
+| fix_e_wf: forall i (es:efnlst), efnlst_wf (2 + i) es ->
+                                     exp_wf i (Fix_e es)
+| proj_e_wf: forall i e n, exp_wf i e -> exp_wf i (Proj_e e n)
+with exps_wf: N -> exps -> Prop :=
+| enil_wf: forall i, exps_wf i enil
+| econs_wf: forall i e es, exp_wf i e -> exps_wf i es -> exps_wf i (econs e es)
+with efnlst_wf: N -> efnlst -> Prop :=
+| flnil_wf_e: forall i, efnlst_wf i eflnil
+| flcons_wf_e: forall i e es, exp_wf i e -> efnlst_wf i es ->
+                           efnlst_wf i (eflcons e es)
+with branches_wf: N -> branches_e -> Prop :=
+| brnil_wf: forall i, branches_wf i brnil_e
+| brcons_wf: forall i d n e bs, exp_wf (n + i) e -> branches_wf i bs ->
+                                branches_wf i (brcons_e d n e bs).
+Hint Constructors exp_wf exps_wf branches_wf.
+Scheme exp_wf_ind2 := Induction for exp_wf Sort Prop
+with exps_wf_ind2 := Induction for exps_wf Sort Prop
+with efnlst_wf_ind2 := Induction for efnlst_wf Sort Prop
+with branches_wf_ind2 := Induction for branches_wf Sort Prop.
+Combined Scheme my_exp_wf_ind from
+         exp_wf_ind2, exps_wf_ind2, efnlst_wf_ind2, branches_wf_ind2.
+
+
+(** Weakening with respect to [exp_wf]. *)
+Lemma weaken_wf' :
+  (forall i e, exp_wf i e -> forall j, i < j -> exp_wf j e) /\
+  (forall i es, exps_wf i es -> forall j, i < j -> exps_wf j es) /\
+  (forall i es, efnlst_wf i es -> forall j, i < j -> efnlst_wf j es) /\
+  (forall i bs, branches_wf i bs -> forall j, i < j -> branches_wf j bs).
+Proof.  
+  apply my_exp_wf_ind; intros; econstructor; auto; try lia; 
+  match goal with
+    | [ H: forall _, _ -> exp_wf _ ?e |- exp_wf _ ?e] => apply H; lia
+    | _ => idtac
+  end.
+  apply (H (2 + j)). lia.
+Qed.
+
+Lemma weaken_wf: forall i e, exp_wf i e -> forall j, i < j -> exp_wf j e.
+  apply (proj1 weaken_wf').
+Qed.
+
+(** We can always weaken a closed expression. *)
+Lemma weaken_closed: forall e i, exp_wf 0 e -> exp_wf i e.
+  intros. destruct i; auto; eapply weaken_wf; eauto; lia.
+Qed.
+
+Lemma weaken_closeds: forall es i, exps_wf 0 es -> exps_wf i es.
+  intros; destruct i; auto; eapply (proj1 (proj2 weaken_wf')); eauto; lia.
+Qed.
+
+Lemma weaken_branches: forall bs i, branches_wf 0 bs -> branches_wf i bs.
+  intros; destruct i; auto; eapply (proj2 (proj2 weaken_wf')); eauto; lia.
+Qed.
+
+Hint Resolve weaken_closed weaken_closeds weaken_branches.
+
+(* optimised *)
+(** Shift all variables [i] equal or above [k] by [n]. *)
+Section SHIFT.
+  Variable shift: N -> N -> exp -> exp.
+  Fixpoint shift_exps' n k bs :=
+    match bs with
+    | enil => enil
+    | econs e es => econs (shift n k e) (shift_exps' n k es)
+    end.
+  Fixpoint shift_efnlst n k bs :=
+    match bs with
+    | eflnil => eflnil
+    | eflcons e es => eflcons (shift n k e) (shift_efnlst n k es)
+    end.
+  Fixpoint shift_branches' n k bs :=
+    match bs with
+    | brnil_e => brnil_e
+    | brcons_e d na e brs => brcons_e d na (shift n (k+na) e) (shift_branches' n k brs)
+    end.
+End SHIFT.
+
+Fixpoint shift n k e := 
+  match e with
+    | Var_e i => Var_e (if lt_dec i k then i else i + n)
+    | App_e e1 e2 => App_e (shift n k e1) (shift n k e2)
+    | Lam_e e' => Lam_e (shift n (1 + k) e')
+    | Con_e d es => Con_e d (shift_exps' shift n k es)
+    | Let_e e1 e2 => Let_e (shift n k e1) (shift n (1 + k) e2)
+    | Match_e e bs => Match_e (shift n k e) (shift_branches' shift n k bs)
+    | Fix_e es => Fix_e (shift_efnlst shift n (2 + k) es)
+    | Proj_e e m => Proj_e (shift n k e) m
+  end.
+
+Definition shifts := shift_exps' shift.
+Definition shift_fns := shift_efnlst shift.
+Definition shift_branches := shift_branches' shift.
+
+Lemma shift_0:
+  (forall d i, shift 0 i d = d) /\
+  (forall es i, shifts 0 i es = es) /\
+  (forall es i, shift_fns 0 i es = es) /\
+  (forall bs i, shift_branches 0 i bs = bs).
+Proof.
+  apply my_exp_ind; simpl; intros; try reflexivity;
+  try (solve[apply f_equal; rewrite H; reflexivity]);
+  try (solve[apply f_equal2; try rewrite H; try rewrite H0; reflexivity]).
+  - if_split. replace (n+0) with n. reflexivity. lia.
+Qed.
+(*
+(* unoptimised *)
+(** Shift all variables [i] equal or above [k] by [1]. *)
+Section SHFT.
+  Variable shft: N -> exp -> exp.
+  Definition shfts' k es := List.map (shft k) es.
+  Definition shft_branch' (k:N) (b:dcon*N*exp) :=
+    br (fun d n e => (d,n,shft (1+k) e)) b.
+  Definition shft_branches' k bs := List.map (shft_branch' k) bs.
+End SHFT.
+
+Fixpoint shft k e := 
+  match e with
+    | Var_e i => Var_e (if lt_dec i k then i else i + 1)
+    | App_e e1 e2 => App_e (shft k e1) (shft k e2)
+    | Lam_e e' => Lam_e (shft (1 + k) e')
+    | Con_e d es => Con_e d (shfts' shft k es)
+    | Let_e e1 e2 => Let_e (shft k e1) (shft (1 + k) e2)
+    | Match_e e bs => Match_e (shft k e) (shft_branches' shft k bs)
+    | Fix_e es => Fix_e (shfts' shft (2 + k) es)
+    | Proj_e e m => Proj_e (shft k e) m
+  end.
+Definition shfts := shfts' shft.
+Definition shft_branch := shft_branch' shft.
+Definition shft_branches := shft_branches' shft.
+
+(* optimised *)
+(** Substitute [v] for variable [k] in [e]. *)
+Section SUBST.
+  Variable subst: exp -> N -> exp -> exp.
+  Definition substs' v k es := List.map (subst v k) es.
+  Definition subst_branch' v k b := br (fun d n e => (d,n,subst v (n+k) e)) b.
+  Definition subst_branches' v k bs := List.map (subst_branch' v k) bs.
+End SUBST.
+  
+Fixpoint subst (v:exp) k (e:exp): exp :=
+  match e with
+    | Var_e i => if lt_dec i k then Var_e i
+                 else if eq_dec i k then shift k 0 v
+                      else Var_e (i - 1)
+    | App_e e1 e2 => App_e (subst v k e1) (subst v k e2)
+    | Lam_e e' => Lam_e (subst v (1 + k) e')
+    | Con_e d es => Con_e d (substs' subst v k es)
+    | Let_e e1 e2 => Let_e (subst v k e1) (subst v (1 + k) e2)
+    | Match_e e bs => Match_e (subst v k e) (subst_branches' subst v k bs)
+    | Fix_e es => Fix_e (substs' subst v (2 + k) es)
+    | Proj_e e m => Proj_e (subst v k e) m
+  end.
+Definition substs := substs' subst.
+Definition subst_branch := subst_branch' subst.
+Definition subst_branches := subst_branches' subst.
+***)
+
+(** Substitute [v] for variable [k] in [e];
+*** no shifting, only for evaluation of closed expressions. *)
+Function sbst (v:exp) k (e:exp): exp :=
+  match e with
+    | Var_e i => if lt_dec i k then Var_e i
+                 else if eq_dec i k then v else Var_e (i - 1)
+    | App_e e1 e2 => App_e (sbst v k e1) (sbst v k e2)
+    | Lam_e e' => Lam_e (sbst v (1 + k) e')
+    | Con_e d es => Con_e d (sbsts v k es)
+    | Let_e e1 e2 => Let_e (sbst v k e1) (sbst v (1 + k) e2)
+    | Match_e e bs => Match_e (sbst v k e) (sbst_branches v k bs)
+    | Fix_e es => Fix_e (sbst_efnlst v (2 + k) es)
+    | Proj_e e m => Proj_e (sbst v k e) m
+  end
+with sbsts (v:exp) k (es:exps) : exps :=
+       match es with
+         | enil => enil
+         | econs f fs => econs (sbst v k f) (sbsts v k fs)
+       end
+with sbst_efnlst (v:exp) k (es:efnlst) : efnlst :=
+       match es with
+         | eflnil => eflnil
+         | eflcons f fs => eflcons (sbst v k f) (sbst_efnlst v k fs)
+       end
+with sbst_branches (v:exp) k (bs:branches_e) : branches_e :=
+       match bs with
+         | brnil_e => brnil_e
+         | brcons_e d n e bs =>
+           brcons_e d n (sbst v (n+k) e) (sbst_branches v k bs)
+       end.
+
+(** Notation for optimised substitution. **
+Class Substitute (v:Type) (t:Type) := { substitute: v -> N -> t -> t }.
+Notation "M { j := N }" := (substitute N j M)
+                      (at level 10, right associativity).
+Instance ExpSubstitute: Substitute exp exp :=
+  { substitute := subst}.
+Instance ExpsSubstitute: Substitute exp (list exp) :=
+  { substitute := substs}.
+Instance BranchSubstitute: Substitute exp (dcon * N * exp) :=
+  { substitute := subst_branch}.
+Instance BranchesSubstitute: Substitute exp (list (dcon * N * exp)) := 
+  { substitute := subst_branches}.
+**)
+
+(** Notation for unoptimised substitution. *)
+Class Sbstitute (v:Type) (t:Type) := { sbstitute: v -> N -> t -> t }.
+Notation "M { j ::= N }" := (sbstitute N j M)
+                      (at level 10, right associativity).
+Instance ExpSbstitute: Sbstitute exp exp :=
+  { sbstitute := sbst}.
+Instance ExpsSbstitute: Sbstitute exp exps :=
+  { sbstitute := sbsts}.
+Instance EfnlstSbstitute: Sbstitute exp efnlst :=
+  { sbstitute := sbst_efnlst}.
+Instance BranchesSbstitute: Sbstitute exp branches_e := 
+  { sbstitute := sbst_branches}.
+
+Lemma Var_e_sbst_inv:
+  forall e j v x, Var_e j = sbst v x e -> exists k, e = Var_e k.
+Proof.
+  induction e; simpl; intros; try discriminate.
+  - exists n. reflexivity.
+Qed.
+
+(* These lemmas come from "A Head-to-Head Comparison of deBruijn
+   Indices and Names" by Stefan Berghofer and Christian Urban. It's
+   notable that they and others remark that coming up with these on
+   your own is quite difficult...
+
+   I don't actually need these yet, so they are not quite up to date
+   with the rest of the development.  *)
+(*
+Lemma shift_twice:
+  forall N i j m n, i <= j -> j <= i + m ->
+ shift n j (shift m i N) = shift (m + n) i N.
+Proof.
+  assert ((forall N i j m n, i <= j -> j <= i + m ->
+ shift n j (shift m i N) = shift (m + n) i N) /\
+          (forall Ns i j m n, i <= j -> j <= i + m ->
+ shifts n j (shifts m i Ns) = shifts (m + n) i Ns)).
+  apply my_exp_ind; intros; simpl; auto ;
+  try (rewrite H; auto; try lia; rewrite H0; auto; try lia; auto).
+  repeat if_split. apply f_equal. lia.
+  tauto.
+Qed.
+
+Lemma shift_subst :
+  forall N i k j L, k <= j ->
+ shift i k (N{j := L}) = (shift i k N){j+i := L}.
+Proof.
+  assert ((forall N i k j L, k <= j ->
+ shift i k (N{j := L}) = (shift i k N){j+i := L}) /\
+          (forall Ns i k j L, k <= j ->
+ shifts i k (Ns{j := L}) = (shifts i k Ns){j+i := L})).
+  apply my_exp_ind; intros; simpl; auto ;
+  try (rewrite H; auto; rewrite H0; auto).
+  repeat if_split. destruct (lt_dec j k); try lia.
+  rewrite shift_twice; auto; lia.
+  destruct (lt_dec n k); try lia; auto. apply f_equal. lia.
+  apply f_equal. rewrite H; try lia. simpl.
+  replace (1 + j + i) with (1 + (j + i)); auto; lia. 
+  tauto.
+Qed.
+
+Lemma shift_away_subst :
+  forall (L:exp) k i j (P:exp), k <= i -> i < k + (j + 1) ->
+                    (shift (1 + j) k L){i := P} = shift j k L.
+Proof.
+  assert ((forall (L:exp) k i j (P:exp), k <= i -> i < k + (j + 1) ->
+                                         (shift (1 + j) k L){i := P} = shift j k L) /\
+          (forall (Ls:exps) k i j (P:exp), k <= i -> i < k + (j + 1) ->
+                                         (shifts (1 + j) k Ls){i := P} = shifts j k Ls)).
+  apply my_exp_ind; simpl; intros; auto ;
+  try (rewrite H; auto; try lia; rewrite H0; auto).
+  repeat if_split. replace (n + (1 + j) - 1) with (n + j); auto; lia.
+  tauto.
+Qed.
+
+(** According to Berghofer and Urban, this is a critical property of substitution,
+    though we don't use it here. *)
+Lemma substitution :
+  forall (M N L:exp) i j, i <= j ->
+    M{i := N}{j := L} = M{1+j := L}{i := N{ j-i := L}}.
+Proof.
+  assert ((forall (M:exp) N L i j, i <= j -> M{i := N}{j := L} = M{1+j := L}{i := N{ j-i := L}}) /\
+          (forall (Ms:exps) N L i j, i <= j -> Ms{i := N}{j := L} = Ms{1+j := L}{i := N{ j-i := L}})).
+  apply my_exp_ind; intros; simpl in *; auto ;
+  try (rewrite H; auto; rewrite H0; auto).
+  repeat if_split.
+  assert (0 <= j - i). lia.
+  generalize (shift_subst N i 0 (j - i) L H0). intros.
+  unfold substitute in H1. simpl in H1.
+  rewrite H1. replace (j - i + i) with j; auto. lia.
+  destruct (eq_dec n 0). lia.
+  generalize  (shift_away_subst L 0 i (n - 1)). intro.
+  unfold substitute in H0. simpl in H0.
+  specialize (H0 (subst L (n - 1 - i) N)). rewrite H0; auto. lia. lia.
+  apply f_equal.
+  rewrite H. replace (1 + j - (1 + i)) with (j - i). auto. lia. lia.
+  tauto.
+Qed.
+*)
+
+Fixpoint sbst_list (e:exp) (vs:exps): exp :=
+  match vs with
+    | enil => e
+    | econs v vs => sbst_list (e{0::=v}) vs
+  end.
+
+(** Find a branch in a match expression corresponding to a given constructor
+    and arity. *)
+Fixpoint find_branch (d:dcon) (m:N) (bs:branches_e) : option exp :=
+  match bs with
+    | brnil_e => None
+    | brcons_e d' n e bs =>
+      if eq_dec d d' then (if eq_dec n m then Some e else None)
+                     else find_branch d m bs
+  end.
+
+(** Big-step evaluation for [exp]. *)
+Inductive eval: exp -> exp -> Prop :=
+| eval_Lam_e: forall e, eval (Lam_e e) (Lam_e e)
+| eval_App_e: forall e1 e1' e2 v2 v,
+                 eval e1 (Lam_e e1') ->
+                 eval e2 v2 ->
+                 eval (e1'{0 ::= v2}) v -> 
+                 eval (App_e e1 e2) v
+| eval_Con_e: forall d es vs, evals es vs -> eval (Con_e d es) (Con_e d vs)
+| eval_Let_e: forall e1 v1 e2 v2,
+                 eval e1 v1 ->
+                 eval (e2{0::=v1}) v2 ->
+                 eval (Let_e e1 e2) v2
+| eval_Match_e: forall e bs d vs e' v,
+                   eval e (Con_e d vs) ->
+                   find_branch d (exps_length vs) bs = Some e' ->
+                   eval (sbst_list e' vs) v ->
+                   eval (Match_e e bs) v
+| eval_Fix_e: forall es, eval (Fix_e es) (Fix_e es)
+| eval_Proj_e: forall e (es:efnlst) n e',
+                  eval e (Fix_e es) ->
+                  enthopt (N.to_nat n) es = Some e' ->
+                  eval (Proj_e e n) ((Lam_e e'){0 ::= Fix_e es})
+with evals: exps -> exps -> Prop :=
+     | evals_nil: evals enil enil
+     | evals_cons: forall e es v vs, eval e v -> evals es vs ->
+                                        evals (econs e es) (econs v vs).
+Scheme eval_ind2 := Induction for eval Sort Prop
+with evals_ind2 := Induction for evals Sort Prop.
+Combined Scheme my_eval_ind from eval_ind2, evals_ind2.
+
+(** some sanity checks of [eval] **)
+Lemma eval_idempotent:
+  (forall e d, eval e d -> eval d d) /\
+  (forall es ds, evals es ds -> evals ds ds).
+Proof.
+  apply my_eval_ind; simpl; intros; try constructor; try assumption.
+Qed.
+
+Lemma eval_single_valued:
+  (forall e d, eval e d -> forall f, eval e f -> d = f) /\
+  (forall es ds, evals es ds -> forall fs, evals es fs -> ds = fs).
+Proof.
+  apply my_eval_ind; simpl; intros.
+  - inversion H. reflexivity.
+  - inversion H2. subst.
+    assert (j0:Lam_e e1' = Lam_e e1'0). { apply H. assumption. }
+    injection j0; intros h0. subst.
+    assert (j1:v2 = v0). { apply H0. assumption. } subst.
+    apply H1. assumption.
+  - inversion H0. subst. apply f_equal2. reflexivity.
+    apply H. assumption.
+  - inversion H1. subst.
+    assert (j0:v1 = v0). { apply H. assumption. }
+    subst. apply H0. assumption.
+  - inversion H1. subst.
+    specialize (H _ H4). injection H; intros h0 h1. subst. clear H.
+    rewrite H5 in e1. injection e1; intros h2. subst. clear e1.
+    apply H0. assumption.
+  - inversion H. subst. reflexivity.
+  - inversion H0. subst. simpl. inversion H0. subst.
+    specialize (H _ H6). injection H; intros h0. subst.
+    rewrite H7 in e1. injection e1; intros h1. subst. reflexivity.
+  - inversion H. reflexivity.
+  - inversion H1. subst. rewrite (H v0); try assumption.
+    rewrite (H0 vs0); try assumption. reflexivity.
+Qed.
+
+
+Example x1: exp := Lam_e (Var_e 0).  (* identity *)
+Lemma Lx1: forall (e d:exp), eval e d -> eval (App_e x1 e) d.
+Proof.
+  intros e d h. unfold x1. eapply eval_App_e. apply eval_Lam_e.
+  apply h. simpl. apply (proj1 eval_idempotent _ _ h).
+Qed.
+
+Example x2: exp := App_e x1 x1.  (* (fun x => x) (fun x => x) *)
+Lemma Lx2: forall (e d:exp), eval e d -> eval (App_e x2 e) d.
+Proof.
+  intros e d h. unfold x2, x1. eapply eval_App_e. 
+  - eapply eval_App_e; try constructor.
+  - eassumption.
+  - simpl. apply (proj1 eval_idempotent _ _ h).
+Qed.
+
+
+(** For testing: a fuel-based interpreter for partial big-step on [exp]. *)
+Function eval_n (n:nat) (e:exp) {struct n}: option exp := 
+  match n with
+    | 0%nat => None
+    | S n => match e with
+               | Lam_e d => Some (Lam_e d)
+               | Fix_e es => Some (Fix_e es)
+               | Con_e d es => 
+                 match evals_n n es with
+                     | None => None
+                     | Some vs => Some (Con_e d vs)
+                 end
+               | App_e e1 e2 =>
+                 match eval_n n e1 with
+                   | Some (Lam_e e1') => 
+                     match eval_n n e2 with
+                       | None => None
+                       | Some e2' => eval_n n (e1'{0 ::= e2'})
+                     end
+                   | _ => None
+                  end
+               | Let_e e1 e2 =>
+                 match eval_n n e1 with
+                   | None => None
+                   | Some v1 => eval_n n (e2{0::=v1})
+                 end
+               | Match_e e bs =>
+                 match eval_n n e with
+                   | Some (Con_e d vs) =>
+                     match find_branch d (exps_length vs) bs with
+                       | None => None
+                       | Some e' => eval_n n (sbst_list e' vs)
+                     end
+                   | _ => None
+                 end
+               | Proj_e e m =>
+                 match eval_n n e with
+                   | Some (Fix_e es) => 
+                     match enthopt (N.to_nat m) es with
+                       | Some e' => Some ((Lam_e e'){0 ::= Fix_e es})
+                       | _ => None
+                     end
+                   | _ => None
+                 end
+               | _ => None
+             end
+  end
+with evals_n n (es:exps) : option exps :=
+       match n with
+         | 0%nat => None
+         | S n => 
+           match es with
+             | enil => Some enil
+             | econs e es => 
+               match (eval_n n e, evals_n n es) with
+                 | (Some v, Some vs) => Some (econs v vs)
+                 | (_, _) => None
+               end
+           end
+       end.
+Functional Scheme eval_n_ind2 := Induction for eval_n Sort Prop
+with evals_n_ind2 := Induction for evals_n Sort Prop.
+Combined Scheme eval_evals_n_ind from eval_n_ind2, evals_n_ind2.
+
+Lemma eval_n_monotone:
+  forall (n:nat) e f, eval_n n e = Some f ->
+                      forall (m:nat), eval_n (n + m) e = Some f.
+Admitted.
+
+Lemma evals_n_monotone:
+  forall (n:nat) es fs, evals_n n es = Some fs ->
+                      forall (m:nat), evals_n (n + m) es = Some fs.
+Admitted.
+
+(***
+Lemma eval_n_weaken:
+  forall (n:nat),
+  (forall e f, eval_n n e = Some f ->
+                 forall m, eval_n (n+m) e = Some f) /\
+  (forall (es:exps) fs, evals_n n es = Some fs ->
+                   forall m, evals_n (n+m) es = Some fs) /\
+  (forall (es:efnlst) fs, evals_n n es = Some fs ->
+                   forall m, evals_n (n+m) es = Some fs). /\
+.
+Proof.
+
+Lemma eval_n_monotone:
+  (forall (n:nat) e f, eval_n n e = Some f -> eval_n (S n) e = Some f).
+Proof.
+  induction n; intros.
+  - simpl; discriminate.
+  - destruct e; simpl; try discriminate; try assumption.
+    destruct (eval_n n e1).
+
+
+
+
+(***
+Lemma eval_n_monotone:
+  forall n:nat,
+  (forall e sf, eval_n n e = sf -> forall f, sf = Some f ->
+                 eval_n (S n) e = Some f) /\
+  (forall es sfs, evals_n n es = sfs -> forall fs, sfs = Some fs ->
+                   evals_n (S n) es = Some fs).
+Proof.
+  intros n.
+  Check (eval_evals_n_ind). 
+           (fun e f =>
+              eval_n n e = Some f -> forall m : nat, eval_n (n + m) e = Some f)).
+***)
+
+Lemma eval_n_monotone:
+  (forall (n:nat) e sf, eval_n n e = sf -> forall f, sf = Some f ->
+                 eval_n (S n) e = Some f).
+Proof.
+  intros n e.
+  functional induction (eval_n n e); intros;
+  try solve [simpl; rewrite <- H0; assumption].
+  - admit.
+  - admit.
+  - 
+
+
+  try discriminate; try assumption.
+  - destruct n0; destruct es.
+    + simpl in e2. discriminate.
+    + simpl in e2. discriminate.
+    + simpl in e2. injection e2; intros h. rewrite h. assumption.
+    + simpl in e2. destruct (eval_n n0 e); destruct (evals_n n0 es).
+
+
+
+Lemma eval_n_monotone:
+  (forall (m n:nat) e f, eval_n n e = Some f ->
+                 eval_n (n+m) e = Some f).
+Proof.
+  induction m; intros n e f h.
+  - replace (n + 0)%nat with n; try omega. assumption.
+  - specialize (IHm (S n)).
+    replace (n + S m)%nat with (S n + m)%nat; try omega.
+    apply IHm.
+
+  functional induction (eval_n n e); simpl; intros;
+  try discriminate; try assumption.
+  - 
+
+
+Lemma eval_n_monotone:
+  (forall n e f, eval_n n e = Some f ->
+                 forall m, (n < m)%nat -> eval_n m e = Some f).
+Proof.
+  intros n e f.
+  functional induction (eval_n n e); intros; try discriminate;
+  assert (h:m = S (m - 1)); try omega; rewrite h; clear h; try assumption.
+  - rewrite <- H.
+    change (evals_n (m - 1) es = Some vs).
+  simpl. injection H; intros h0. rewrite <- h0. 
+
+ simpl. reflexivity.
+
+
+Lemma eval_n_monotone:
+  (forall n e f, eval_n n e = Some f ->
+                 forall m, eval_n (n+m) e = Some f).
+Proof.
+  intros n e f.
+  functional induction (eval_n n e); simpl; intros;
+  try discriminate; try assumption.
+  - 
+
+
+
+  apply (eval_n_ind
+           (fun n e oe =>
+              forall (f:exp), oe = Some f ->
+                              forall m : nat, eval_n (n + m) e = Some f));
+    simpl; intros; try discriminate; try assumption.
+  - 
+
+Lemma eval_n_weaken:
+  (forall n e f, eval_n n e = Some f ->
+                 forall m, eval_n (n+m) e = Some f) /\
+  (forall n es fs, evals_n n es = Some fs ->
+                   forall m, evals_n (n+m) es = Some fs).
+Proof.
+  Check eval_n_ind.
+  Check (eval_evals_n_ind). 
+           (fun n e f =>
+              eval_n n e = Some f -> forall m : nat, eval_n (n + m) e = Some f)).
+***********)
+
+
+(** [eval_n] is sound w.r.t. [eval] **)
+Lemma eval_n_Some_Succ:
+  forall e (n:nat) v, eval_n n e = Some v -> n = (S (n - 1))%nat.
+Proof.
+  induction n; intros.
+  - simpl in H. discriminate.
+  - omega.
+Qed.
+Lemma evals_n_Some_Succ:
+  forall es (n:nat) vs, evals_n n es = Some vs -> n = (S (n - 1))%nat.
+Proof.
+  induction n; intros.
+  - simpl in H. discriminate.
+  - omega.
+Qed.
+
+Lemma evaln_eval: 
+  forall (n:nat),
+  (forall (e:exp) v, eval_n n e = Some v -> eval e v) /\
+  (forall (es:exps) vs, evals_n n es = Some vs -> evals es vs).
+Proof.
+  apply (eval_evals_n_ind (fun n e ov => forall v, ov = Some v -> eval e v)
+        (fun n es ovs => forall vs, ovs = Some vs -> evals es vs));
+  intros; try discriminate.
+  + injection H; intros h0. subst. constructor.
+  + injection H; intros h0. subst. constructor.
+  + injection H0; intros h0. rewrite <- h0. constructor. apply H. assumption.
+  + econstructor.
+    * specialize (H _ e4). eapply H.
+    * specialize (H0 _ e5). eapply H0.
+    * specialize (H1 _ H2). apply H1.
+  + econstructor.
+    * specialize (H _ e4). eapply H.
+    * specialize (H0 _ H1). apply H0.
+  + econstructor.
+    * specialize (H _ e3). eapply H.
+    * eapply e4. 
+    * specialize (H0 _ H1). apply H0.
+  + injection H0; intros h0. subst. constructor.
+    * apply H. assumption.
+    * assumption.
+  + injection H; intros h0. subst. constructor.
+  + injection H1; intros h0. subst. constructor.
+    * apply H. assumption.
+    * apply H0. assumption.
+Qed.
+
+
+(** [eval_n] is complete w.r.t. [eval] **)
+Lemma eval_evaln:
+  (forall (e v:exp), eval e v -> exists (n:nat), eval_n n e = Some v) /\
+  (forall (es vs:exps), evals es vs -> exists (n:nat), evals_n n es = Some vs).
+Proof.
+  apply my_eval_ind; intros; try (solve [exists 1%nat; reflexivity]).
+  - destruct H as [x h]. destruct H0 as [x0 h0]. destruct H1 as [x1 h1].
+    exists (x+x0+x1)%nat.
+    assert (j:=eval_n_Some_Succ _ _ _ h).
+    assert (j0:=eval_n_Some_Succ _ _ _ h0).
+    assert (j1:=eval_n_Some_Succ _ _ _ h1).
+    assert (k:= eval_n_monotone _ _ _ h).
+    assert (k0:= eval_n_monotone _ _ _ h0).
+    assert (k1:= eval_n_monotone _ _ _ h1).
+    rewrite j.
+    replace (S (x - 1) + x0 + x1)%nat
+    with (S (x + (x0 + x1 - 1)))%nat; try lia.
+    simpl. rewrite k.
+    replace (x + (x0 + x1 - 1))%nat with (x0 + (x + x1 - 1))%nat; try lia.
+    rewrite k0.
+    replace (x0 + (x + x1 - 1))%nat with (x1 + (x + x0 - 1))%nat; try lia.
+    rewrite k1. reflexivity.
+  - destruct H as [x h]. exists (x+1)%nat.
+    assert (j:=evals_n_Some_Succ _ _ _ h).
+    assert (k:= evals_n_monotone _ _ _ h).
+    rewrite j.
+    replace (S (x - 1) + 1)%nat with (S (x + 0))%nat; try lia.
+    simpl. rewrite k. reflexivity.
+  - destruct H as [x h]. destruct H0 as [x0 h0].
+    assert (j:=eval_n_Some_Succ _ _ _ h).
+    assert (j0:=eval_n_Some_Succ _ _ _ h0).
+    assert (k:= eval_n_monotone _ _ _ h).
+    assert (k0:= eval_n_monotone _ _ _ h0).
+    exists (x+x0)%nat.
+    rewrite j.
+    replace (S (x - 1) + x0)%nat with (S (x + (x0 - 1)))%nat; try lia.
+    simpl. rewrite k.
+    replace (x + (x0 - 1))%nat with (x0 + (x - 1))%nat; try lia.
+    rewrite k0. reflexivity.
+  - destruct H as [x h]. destruct H0 as [x0 h0].
+    assert (j:=eval_n_Some_Succ _ _ _ h).
+    assert (j0:=eval_n_Some_Succ _ _ _ h0).
+    assert (k:= eval_n_monotone _ _ _ h).
+    assert (k0:= eval_n_monotone _ _ _ h0).
+    exists (x+x0)%nat.
+    rewrite j.
+    replace (S (x - 1) + x0)%nat with (S (x + (x0 - 1)))%nat; try lia.
+    simpl. rewrite k.
+    replace (x + (x0 - 1))%nat with (x0 + (x - 1))%nat; try lia.
+    rewrite e1. rewrite k0. reflexivity.
+  - destruct H as [x h]. exists (x+1)%nat.
+    assert (j:=eval_n_Some_Succ _ _ _ h).
+    assert (k:= eval_n_monotone _ _ _ h).
+    rewrite j.
+    replace (S (x - 1) + 1)%nat with (S (x + 0))%nat; try lia.
+    simpl. rewrite k. rewrite e1. reflexivity.
+  - destruct H as [x h]. destruct H0 as [x0 h0].
+    assert (j:=eval_n_Some_Succ _ _ _ h).
+    assert (j0:=evals_n_Some_Succ _ _ _ h0).
+    assert (k:= eval_n_monotone _ _ _ h).
+    assert (k0:= evals_n_monotone _ _ _ h0).
+    exists (x+x0)%nat.
+    rewrite j.
+    replace (S (x - 1) + x0)%nat with (S (x + (x0 - 1)))%nat; try lia.
+    simpl. rewrite k.
+    replace (x + (x0 - 1))%nat with (x0 + (x - 1))%nat; try lia.
+    rewrite k0. reflexivity.
+Qed.
+
+
+(** some concrete examples **)
+Example Ke: exp := Lam_e (Lam_e (Var_e 1)).
+Example Se: exp := Lam_e (Lam_e (Lam_e
+            (App_e (App_e (Var_e 2) (Var_e 0)) (App_e (Var_e 1) (Var_e 0))))).
+Example SKKe: exp := App_e (App_e Se Ke) Ke.
+Eval vm_compute in (eval_n 1000 (App_e SKKe (Con_e 10 enil))).
+Goal eval (App_e SKKe (Con_e 10 enil)) (Con_e 10 enil).
+Proof.
+  unfold SKKe, Se, Ke. repeat econstructor.
+Qed.
+
+Infix "$" := App_e   (at level 201, left associativity).
+Definition Ve0 := (Var_e 0).
+Definition Ve1 := (Var_e 1).
+Definition Ve2 := (Var_e 2).
+Definition Ve3 := (Var_e 3).
+Definition Ve4 := (Var_e 4).
+Definition Ve5 := (Var_e 5).
+
+Definition unsome (x:option exp) : exp :=
+  match x with 
+    | Some e => e
+    | None => Var_e 9999
+  end.
+
+(** natural numbers in Church representation **)
+Section ChurchNaturals.
+Notation ZZ := (Lam_e (Lam_e Ve1)).
+Notation SS := (Lam_e (Lam_e (Lam_e (Ve0 $ (Ve2 $ Ve1 $ Ve0))))).
+Notation one := (SS $ ZZ).
+Notation two := (SS $ one).
+Notation three := (SS $ two).
+Notation four := (SS $ three).
+Notation five := (SS $ four).
+Notation six := (SS $ five).
+Notation add := (Lam_e (Lam_e (Ve1 $ Ve0 $ SS))).
+Notation mul := (Lam_e (Lam_e (Ve1 $ ZZ $ (add $ Ve0)))).
+
+Example One := Eval compute in (unsome (eval_n 100 one)).
+Example Two := Eval compute in (unsome (eval_n 100 two)).
+Example Three := Eval vm_compute in (unsome (eval_n 100 three)).
+Example Four := Eval vm_compute in (unsome (eval_n 100 four)).
+Example Five := Eval vm_compute in (unsome (eval_n 100 five)).
+Example Six := Eval vm_compute in (unsome (eval_n 100 six)).
+
+Goal eval (SS $ ZZ) One. repeat econstructor. Qed.
+Goal eval (add $ ZZ $ one) One. repeat econstructor. Qed.
+Goal eval (add $ one $ ZZ) One. repeat econstructor. Qed.
+Goal (eval_n 1000 (add $ two $ one)) = Some Three.
+vm_compute. reflexivity. Qed.
+Goal (eval_n 1000 (add $ two $ three)) = Some Five.
+vm_compute. reflexivity. Qed.
+Goal (eval_n 1000 (mul $ two $ three)) = Some Six.
+vm_compute. reflexivity. Qed.
+End ChurchNaturals.
+Reset ChurchNaturals.
+
+(** booleans using native data constructors (with no arguments) **)
+Notation TT := (0:dcon).
+Notation TTT := (Con_e TT enil).
+Notation FF := (1:dcon).
+Notation FFF := (Con_e FF enil).
+(* if b then e1 else e2 *)
+Notation ite :=
+  (Lam_e (Lam_e (Lam_e
+             (Match_e Ve2 (brcons_e TT 0 Ve1 (brcons_e FF 0 Ve0 brnil_e)))))).
+Goal eval (ite $ TTT $ FFF $ TTT) FFF.
+repeat econstructor. Qed.
+Goal eval (ite $ FFF $ FFF $ TTT) TTT.
+repeat econstructor. Qed.
+
+(** lists using native data constructors: Cons takes 2 arguments **)
+Notation dNil := (2:dcon).
+Notation Nil := (Con_e dNil enil).
+Notation dCons := (3:dcon).
+Notation Cons := (Lam_e (Lam_e (Con_e dCons (econs Ve1 [|Ve0|])))).
+Notation cdr :=
+  (Lam_e (Match_e Ve0 (brcons_e dNil 0 Nil (brcons_e dCons 2 Ve1 brnil_e)))).
+
+Goal eval (cdr $ Nil) Nil.
+eapply eval_App_e.
+- eapply eval_Lam_e.
+- eapply eval_Con_e. eapply evals_nil.
+- eapply eval_Match_e.
+  + compute. eapply eval_Con_e. eapply evals_nil.
+  + compute. apply f_equal. reflexivity.
+  + compute. eapply eval_Con_e. eapply evals_nil.
+Qed.
+
+(* test match on a data constructor with an argument *)
+Goal eval (cdr $ (Cons $ TTT $ Nil)) Nil.
+repeat (try econstructor; try vm_compute).
+Qed.
+
+Goal eval (Cons $ TTT $ Nil)
+     (Con_e dCons (econs (Con_e TT enil) [|Con_e dNil enil|])).
+repeat (try econstructor; try vm_compute).
+Qed.
+Goal eval (cdr $ (Cons $ FFF $ (Cons $ TTT $ Nil)))
+     (Con_e dCons (econs (Con_e TT enil) [|Con_e dNil enil|])).
+repeat (try econstructor; try vm_compute).
+Qed.
+
+
+(** Natural numbers using native data constructors **)
+Notation ZZ := (0:dcon).
+Notation ZZZ := (Con_e ZZ enil).
+Notation SS := (1:dcon).
+Notation SSS := (Lam_e (Con_e SS [|Ve0|])).
+Notation one := (SSS $ ZZZ).
+Notation two := (SSS $ one).
+Notation three := (SSS $ two).
+Notation four := (SSS $ three).
+Notation five := (SSS $ four).
+Notation six := (SSS $ five).
+
+Example One := Eval compute in (unsome (eval_n 1000 one)).
+Print One.
+Example Two := Eval compute in (unsome (eval_n 100 two)).
+Example Three := Eval vm_compute in (unsome (eval_n 100 three)).
+Example Four := Eval vm_compute in (unsome (eval_n 100 four)).
+Example Five := Eval vm_compute in (unsome (eval_n 100 five)).
+Example Six := Eval vm_compute in (unsome (eval_n 100 six)).
+
+Goal eval (SSS $ one) Two.
+repeat econstructor. 
+Qed.
+
+Goal eval (SSS $ three) Four.
+repeat econstructor. 
+Qed.
+
+(** fixpoints **)
+Definition pre_copy : exp :=
+  (Fix_e [!(Match_e Ve0 (brcons_e ZZ 0 ZZZ 
+            (brcons_e SS 1 (SSS $ ((Proj_e Ve2 0) $ Ve0)) brnil_e)))!]).
+Definition copy :exp := Proj_e pre_copy 0.
+
+Goal eval (copy $ ZZZ) ZZZ.
+unfold copy, pre_copy.
+repeat (try econstructor; try vm_compute).
+Qed.
+
+Eval vm_compute in eval_n 100 (copy $ six).
+
+
+(**** Fixpoints???  ****
+Goal eval (copy $ one) One.
+unfold copy. eapply eval_App_e.
+- eapply eval_Lam_e. 
+- eapply eval_App_e.
+  + eapply eval_Lam_e. 
+  + repeat econstructor.
+  + simpl. eapply eval_Con_e. repeat econstructor.
+- vm_compute. eapply eval_Match_e.
+  + eapply eval_Con_e. repeat econstructor.
+  + unfold find_branch. repeat if_split. 
+    * discriminate.
+    * apply f_equal. eapply eval_Proj_e.
+    
+
+repeat (try econstructor; try vm_compute).
+Qed.
+
+Definition copy : exp :=
+  Lam_e (Fix_e ((eflcons (Match_e Ve1
+                            (brcons_e ZZ 0 ZZZ
+                                      (brcons_e SS 1 (Proj_e Ve0 1) brnil_e))) eflnil))).
+
+Goal eval (copy $ ZZZ) ZZZ.
+repeat (try econstructor; try vm_compute).
+
+
+Definition add :=
+  (Lam_e (Lam_e (Proj (Fix_e
+                   (eflcons (Match_e Ve1
+                            (brcons_e ZZ 0 Ve0
+                                      (brcons_e SS 1
+                                                (Proj_e SSS 0) brnil_e)))
+                            eflnil)))).
+
+Goal eval (add $ ZZZ $ ZZZ) ZZZ.
+unfold add. eapply eval_App_e. 
+- eapply eval_App_e.
+  + eapply eval_Lam_e. 
+  + eapply eval_Con_e. constructor.
+  + eapply eval_Lam_e.
+- eapply eval_Con_e. constructor.
+- vm_compute. eapply eval_Fix_e.
+
+
+Goal eval one (Con_e SS [|ZZZ|]).
+eapply eval_App_e.
+eapply eval_Lam_e.
+eapply eval_Con_e. eapply evals_nil.
+simpl. eapply eval_Con_e. eapply evals_cons.
+eapply eval_Con_e. eapply evals_nil. eapply evals_nil.
+Qed.
+
+Example One := Eval compute in (unsome (eval_n 1000 one)). 
+Example Two := Eval compute in (unsome (eval_n 100 two)).
+Example Three := Eval vm_compute in (unsome (eval_n 100 three)).
+Example Four := Eval vm_compute in (unsome (eval_n 100 four)).
+Example Five := Eval vm_compute in (unsome (eval_n 100 five)).
+Example Six := Eval vm_compute in (unsome (eval_n 100 six)).
+
+
+
+(** If [e] is an [i+1] expression, and [v] is a closed expression, then 
+    for any [k <= i], substituting [v] for [k] in e yields an [i] expression.
+
+    I wish I could generalize this to non-closed expressions, but haven't
+    been able to.  But perhaps the whole point is that I need to shift [v]
+    or something.
+ *)
+Lemma sbst_preserves_wf' :
+  (forall i' e, exp_wf i' e ->
+     forall i, i' = 1 + i -> forall v, exp_wf 0 v ->
+       forall k, k <= i -> exp_wf i (e{k::=v})) /\
+  (forall i' es, exps_wf i' es ->
+     forall i, i' = 1 + i -> forall v, exp_wf 0 v ->
+       forall k, k <= i -> exps_wf i (es{k::=v})) /\
+  (forall i' es, efnlst_wf i' es ->
+     forall i, i' = 1 + i -> forall v, exp_wf 0 v ->
+       forall k, k <= i -> efnlst_wf i (es{k::=v})) /\
+  (forall i' bs, branches_wf i' bs ->
+     forall i, i' = 1 + i -> forall v, exp_wf 0 v ->
+       forall k, k <= i -> branches_wf i (bs{k::=v})).
+Proof.
+  apply my_exp_wf_ind; simpl; intros; subst; eauto.
+  - repeat if_split; try (constructor; auto; lia).
+  - constructor. apply H; try lia; auto.
+  - constructor; auto. apply H0; try lia; auto.
+  - constructor; auto. apply H; try lia; auto.
+  - constructor; auto. 
+  - constructor; auto. 
+  - constructor; auto. apply H; try lia; auto.
+Qed.
+
+(** Corrollary:  if [e] is an [i+1] expression, and [v] is closed, then 
+   substituting [v] for [0] in [e] yields an [i] expression. *)
+Lemma sbst_preserves_exp_wf :
+  forall i e, exp_wf (1 + i) e -> forall v, exp_wf 0 v ->
+                                            exp_wf i (e {0::= v}).
+Proof.
+  intros. eapply (proj1 sbst_preserves_wf'); eauto; lia.
+Qed.
+
+Lemma subst_list_preserves_exp_wf :
+  forall vs, exps_wf 0 vs -> 
+             forall i e, exp_wf ((exps_length vs) + i) e ->
+                         exp_wf i (sbst_list e vs).
+Proof.
+  induction vs; simpl; intros; subst; auto. 
+  inversion H; clear H; subst.
+  replace (1 + exps_length vs + i) with (1 + (exps_length vs + i)) in H0;
+    try lia.
+  apply IHvs; auto. apply sbst_preserves_exp_wf; auto.
+Qed.
+  
+Lemma sbst_preserves_exps_wf :
+  forall i es, exps_wf (1 + i) es -> 
+               forall v, exp_wf 0 v -> exps_wf i (es {0 ::= v}).
+Proof.
+  intros. eapply (proj1 (proj2 sbst_preserves_wf')); eauto; lia.
+Qed.
+Lemma sbst_preserves_branches_wf :
+  forall i bs, branches_wf (1 + i) bs ->
+               forall v, exp_wf 0 v -> branches_wf i (bs {0 ::= v}).
+Proof.
+  intros; eapply (proj2 (proj2 sbst_preserves_wf')); eauto; lia.
+Qed.
+Hint Resolve sbst_preserves_exp_wf sbst_preserves_exps_wf 
+     sbst_preserves_branches_wf.
+
+Lemma nthopt_preserves_wf :
+  forall i es, efnlst_wf i es ->
+               forall n e, enthopt n es = Some e -> exp_wf i e.
+Proof.
+  induction es; simpl; intros. 
+  - destruct n; discriminate.
+  - inversion H; subst. destruct n; simpl in *.
+    + injection H0; intros; subst; auto. 
+    + specialize (IHes H5 n e0).
+      apply IHes. auto.
+Qed.
+
+Lemma find_branch_preserves_wf :
+  forall i bs, branches_wf i bs ->
+               forall d m e, find_branch d m bs = Some e -> exp_wf (m+i) e.
+Proof.
+  induction 1; simpl; intros a b c; repeat if_split; intro H1;
+  try discriminate.
+  - injection H1; intros; subst; auto. 
+  - eapply IHbranches_wf; eauto.
+Qed.
+Hint Resolve find_branch_preserves_wf.
+
+(** Evaluation preserves closed expressions.  I wish I could generalize this
+   to evaluation preserves [i] expressions. *)
+Lemma eval_preserves_wf' :
+  (forall e v, eval e v -> exp_wf 0 e -> exp_wf 0 v) /\
+  (forall es vs, evals es vs -> exps_wf 0 es -> exps_wf 0 vs).
+Proof.
+  apply my_eval_ind; simpl; intros; auto.
+  - inversion H2; clear H2; subst.
+    specialize (H H6); clear H6. specialize (H0 H7); clear H7.
+    inversion H; clear H; subst. apply H1; auto. 
+  - inversion H0; auto. 
+  - inversion H1; auto.
+  - inversion H1; clear H1; subst. apply H0; auto.
+    apply subst_list_preserves_exp_wf. specialize (H H5). inversion H; subst.
+    auto. eapply find_branch_preserves_wf; eauto.
+  - inversion H0; subst. clear H0.
+    specialize (H H3). inversion H; subst.
+    apply (fun H' => sbst_preserves_exp_wf 0 (Lam_e e') H' (Fix_e es) H).
+    constructor.  eapply nthopt_preserves_wf; eassumption.
+  - inversion H1; subst. constructor; auto.
+Qed.
+Definition eval_preserves_wf := proj1 eval_preserves_wf'.
+Definition evals_preserves_wf := proj2 eval_preserves_wf'.
+
+(** Characterize values **)
+Inductive is_value: exp -> Prop :=
+| var_is_value: forall i, is_value (Var_e i)
+| lam_is_value: forall e, is_value (Lam_e e)
+| con_is_value: forall d es, are_values es -> is_value (Con_e d es)
+| fix_is_value: forall es, is_value (Fix_e es)
+with are_values: exps -> Prop :=
+| enil_are_values: are_values enil
+| econs_are_values: forall e es, is_value e -> are_values es ->
+                                 are_values (econs e es).
+Scheme is_value_ind2 := Induction for is_value Sort Prop
+with are_values_ind2 := Induction for are_values Sort Prop.
+Combined Scheme my_is_value_ind from is_value_ind2, are_values_ind2.
+Hint Constructors is_value are_values.
+
+(** Show that evaluation always yields a value. *)
+Lemma eval_yields_value' :
+  (forall e v, eval e v -> is_value v) /\
+  (forall es vs, evals es vs -> are_values vs).
+Proof.
+  apply my_eval_ind; simpl; intros; auto; try constructor; auto.
+Qed.
+Definition eval_yields_value := proj1 eval_yields_value'.
+Definition evals_yields_values := proj2 eval_yields_value'.
+Hint Resolve eval_yields_value evals_yields_values.
+
+(** Computable test as to whether a source expression is already a
+    value (a.k.a., atomic).  *)
+Fixpoint is_valueb (e:exp): bool :=
+  match e with
+    | Var_e _ => true
+    | Lam_e _ => true
+    | App_e _ _  => false
+    | Con_e _ es => are_valuesb es
+    | Match_e _ _ => false
+    | Let_e _ _ => false
+    | Fix_e _ => true
+    | Proj_e _ _ => false
+  end
+with are_valuesb (es:exps): bool :=
+       match es with
+         | enil => true
+         | econs f fs => if is_valueb f then are_valuesb fs else false
+       end.
+
+Lemma is_valueb_corr' :
+  (forall e, is_valueb e = true <-> is_value e) /\
+  (forall es, are_valuesb es = true <-> are_values es) /\
+  (forall (es:efnlst), True) /\
+  (forall (bs:branches_e), True).
+Proof.
+  apply my_exp_ind; simpl; intros; split; intros; auto;
+  try discriminate; try inversion H1.
+  - constructor. rewrite <- H. auto.
+  - inversion H0; subst. rewrite H. auto.
+  - inversion H0; try discriminate.
+  - destruct (is_valueb e); try discriminate. constructor.
+    + apply H; auto.
+    + apply H0; auto. 
+  - inversion H1; subst. destruct (is_valueb e). 
+    + tauto. 
+    + apply H. auto.
+Qed.
+Definition is_valueb_corr := proj1 is_valueb_corr'.
+Definition are_valuesb_corr := proj1 (proj2 is_valueb_corr').
+Hint Rewrite is_valueb_corr.
+Hint Rewrite are_valuesb_corr.
+Hint Resolve is_valueb_corr.
+Hint Resolve are_valuesb_corr.
+
+Fixpoint exps_append (es1 es2:exps) : exps :=
+  match es1 with
+    | enil => es2
+    | econs e es => econs e (exps_append es es2)
+  end.
+Lemma exps_append_enil_r:
+  forall (es:exps), exps_append es enil = es.
+Proof.
+  induction es; simpl. reflexivity. rewrite IHes. reflexivity.
+Qed.
+
+Lemma are_values_append :
+  forall es1 es2, (are_values es1 /\ are_values es2) <->
+                  are_values (exps_append es1 es2).
+Proof.
+  induction es1 ; simpl ; intros ; split ; intro.
+  - destruct H ; auto.
+  - destruct H ; auto.
+  - destruct H. inversion H. subst. constructor ; auto. rewrite <- IHes1. auto.
+  - inversion H ; subst. rewrite <- IHes1 in H3. destruct H3. split ; auto.
+Qed.
+Hint Resolve are_values_append.
+
+***************)
